## Sin/Cos

![[Bildschirmfoto 2024-09-24 um 23.41.35.png]]

$f(x) = \sin(x) -> f'(x) = \cos(x)$
$f(x) = \cos(x) -> f'(x) = -\sin(x)$
$f(x) = -\sin(x) -> f'(x) = -\cos(x)$
$f(x) = -\cos(x) -> f'(x) = \sin(x)$
#### Summenregel

$$
(f+g)' = f'+g'
$$

$$
\begin{align}
f(x) &= 2x^2 +3x \\
f'(x) &= 4x +3
\end{align}
$$

#### Produktregel

$$
(f \cdot g)' = f'\cdot g + f\cdot g'
$$

$$
\begin{align}
f(x) &= 2x^4 \cdot 2x^5 \\
f'(x) &= (8x^3 \cdot 2x^5) + (2x^4 +10x^4)   \\
&=8x^3 + 2x^5 + 12x^4
\end{align}
$$

#### Quotientenregel

$$
(\frac{f}{g})' = \frac{(f' \cdot g - f \cdot g')}{g^2}
$$
$$
\begin{align}
f(x) &= \frac{2x^2}{y} \\
f'(x) &= \frac{4x \cdot y - 2x^2 \cdot 2g}{y^2}
\end{align}
$$

#### Kettenregel

$$
(f \circ g)' = (f' \circ g) \cdot g'
$$

#### Konstantenregel


## Extremstellen

$$
\begin{align}
f(x) &= -2x^3 - 12x^2 + 30x + 12 \\
f'(x) &= -6x^2 - 24x + 30 \\
f''(x) &= -12x - 24 \\ \\
& \text{Wir setzen f' = 0} \\ \\
0 &= -6x^2 - 24x + 30 & | :(-6)  \\
0 &= x^2 + 4x - 5 \\ \\
& \text{Wir nutzen die PQ-Formel f√ºr x} \\ \\
x_{1,2} &= -\frac{4}{2} \pm \sqrt{ 4 + 5 } \\
x_{1,2} &= -2 \pm 3  = (1,- 5)
\end{align}
$$




