- https://hpi.de/friedrich/docs/scripts/24_Vorkurs/LineareGleichungssysteme.html
- https://github.com/tyronfranzke/HPI-Vorkurs-2024/blob/main/woche-1/tag-3/aufgaben.pdf

## Aufgabe 1: LGS - 1
(1)

$$
 \begin{align} \\
 2x +10y &= 12x  \\
x+y-12 &= y+6   \\ \\

y &= x  \\
x&=18   \\ \\

&\underline{x=18; y=18 } \\ \\
\text{Probe: } 2\cdot 18 + 10 \cdot 18 &= 12 \cdot 16 \text{ und } 18 + 18 - 12 = 18 +6 \\
 
 \end{align}
$$

## Aufgabe 5: LGS - 3

(1)

$$
\begin{align}
\mathrm{(i)}   &  & 3x - y + z &= 10.5 && | \cdot 2 \\
\mathrm{(ii)}  &  & x + \frac{y}{3} - z &= \frac{25}{6} && | \cdot 6 \\
\mathrm{(iii)}  &  & 7x -3z &= 26.5 \\
\mathrm{(iv)}  &  & \frac{x}{15} + \frac{y}{3} - \frac{z}{9} &= \frac{79}{90} && | \cdot 90 \\
\end{align}
$$

(2)

$$
\begin{align}
\mathrm{(i)}  &  &  z &= 2x + 3y + 6.5  &  & | - 2x  \\
\mathrm{(ii)}  &  &  \frac{y}{2} + z &= x + \frac{43}{4}  &  & | \cdot 4  \\
\mathrm{(iii)} &  & 4z + 3y - 33 &= 5y  &  & |+33  \\
 \\
\mathrm{(i)}  &  &  z -2x &=  3y + 6.5  &  &  | -3y \\
\mathrm{(ii)}  &  &  2y + 4z &= 4x + 43  &  & | -4x  \\
\mathrm{(iii)} &  & 4z + 3y  &= 5y +33  &  &  | -5y \\ 
 \\
\mathrm{(i)}  &  & -2x   -3y +z &=   6.5  &  &  \\
\mathrm{(ii)}  &  &  -4x + 2y + 4z &=  43  &  &  \\
\mathrm{(iii)} &  & 0x -2y + 4z   &= 33  &  &   \\

\end{align}
$$

$$
\begin{pmatrix}
-2 & -3 & 1 & | & 6.5 \\ 
-4 & 2  & 4 & | & 43  \\
0 & -2 & 4 & | & 33 \\
\end{pmatrix}
$$


 $\text{Zeile }2 - 2 \times \text{Zeile } 1$


$$
\begin{pmatrix}
-2 & -3 & 1 & | & 6.5 \\ 
0 & 8  & 2 & | & 30  \\
0 & -2 & 4 & | & 33 \\
\end{pmatrix}
$$


 $\text{Zeile }3 + \frac{1}{4} \times \text{Zeile } 2$


$$
\begin{pmatrix}
-2 & -3 & 1 & | & 6.5 \\ 
0  & 8  & 2 & | & 30  \\
0  & 0 & 4.5 & | & 40.5 \\
\end{pmatrix}
$$


$$
\begin{align}
4.5z &= 40.5 && | :4.5 \\
z &= 9 \\
 \\
8y + 2\cdot 9 &= 30 && | - 18 \\ 
8y &= 12 && | :8 \\
y &= 1.5  \\
 \\
-2x -3\cdot 1.5 + 9 &= 6.5&& | - 4,5 \\ \\
-2x &= 2 && | :(-2) \\
x &= -1
\end{align}
$$

(3)

$$
\begin{align}
\mathrm{(i)}  &  &  \frac{x}{5} +y &= \frac{x}{2} + \frac{9}{30} \\
\mathrm{(ii)}  &  &  z - 3y + \frac{37}{35} &= 0\\
\mathrm{(iii)} &  & y - \frac{19}{15} &= x - \frac{56}{5}z +y &  & \\
\end{align}
$$